book/FPLean/Monads/IO.lean
@@ -112,73 +112,67 @@ Peeling back another layer, {anchorName names}`EIO` is itself defined in terms o
 ```
 ```anchorInfo printEIO
 def EIO : Type → Type → Type :=
-fun ε => EStateM ε IO.RealWorld
+fun ε α => EST ε IO.RealWorld α
 ```
-The {anchorName printEStateM}`EStateM` monad includes both errors and state—it's a combination of {anchorName names}`Except` and {anchorName State (module := Examples.Monads)}`State`.
-It is defined using another type, {anchorName printEStateMResult}`EStateM.Result`:
+The {anchorName printEStateM}`EST` monad includes both errors and state—it's similar to a combination of {anchorName names}`Except` and {anchorName State (module := Examples.Monads)}`State`.
+It is defined using another type, {anchorName printEStateMResult}`EST.Out`:
 ```anchor printEStateM
-#print EStateM
+#print EST
 ```
 ```anchorInfo printEStateM
-def EStateM.{u} : Type u → Type u → Type u → Type u :=
-fun ε σ α => σ → EStateM.Result ε σ α
+def EST : Type → Type → Type → Type :=
+fun ε σ α => Void σ → EST.Out ε σ α
 ```
-In other words, a program with type {anchorTerm EStateMNames}`EStateM ε σ α` is a function that accepts an initial state of type {anchorName EStateMNames}`σ` and returns an {anchorTerm EStateMNames}`EStateM.Result ε σ α`.
+In other words, a program with type {anchorTerm EStateMNames}`EST ε σ α` is a function that accepts an initial state of type {anchorName EStateMNames}`σ` and returns an {anchorTerm EStateMNames}`EST.Out ε σ α`.
+The state is wrapped in the type {anchorName VoidSigma}`Void`, which is an internal primitive that causes a value to be erased from compiled code; {anchorTerm VoidSigma}`Void σ` has the same representation as {anchorName save (module:=Examples.Monads)}`Unit`.
 
-{anchorName EStateMNames}`EStateM.Result` is very much like the definition of {anchorName names}`Except`, with one constructor that indicates a successful termination and one constructor that indicates an error:
+{anchorName EStateMNames}`EST.Out` is very much like the definition of {anchorName names}`Except`, with one constructor that indicates a successful termination and one constructor that indicates an error:
 ```anchor printEStateMResult
-#print EStateM.Result
+#print EST.Out
 ```
 ```anchorInfo printEStateMResult
-inductive EStateM.Result.{u} : Type u → Type u → Type u → Type u
+inductive EST.Out : Type → Type → Type → Type
 number of parameters: 3
 constructors:
-EStateM.Result.ok : {ε σ α : Type u} → α → σ → EStateM.Result ε σ α
-EStateM.Result.error : {ε σ α : Type u} → ε → σ → EStateM.Result ε σ α
+EST.Out.ok : {ε σ α : Type} → α → Void σ → EST.Out ε σ α
+EST.Out.error : {ε σ α : Type} → ε → Void σ → EST.Out ε σ α
 ```
-Just like {anchorTerm Except (module:=Examples.Monads)}`Except ε α`, the {anchorName names (show := ok)}`EStateM.Result.ok` constructor includes a result of type {anchorName Except (module:=Examples.Monads)}`α`, and the {anchorName names (show := error)}`EStateM.Result.error` constructor includes an exception of type {anchorName Except (module:=Examples.Monads)}`ε`.
+Just like {anchorTerm Except (module:=Examples.Monads)}`Except ε α`, the {anchorName names (show := ok)}`EST.Out.ok` constructor includes a result of type {anchorName Except (module:=Examples.Monads)}`α`, and the {anchorName names (show := error)}`EST.Out.error` constructor includes an exception of type {anchorName Except (module:=Examples.Monads)}`ε`.
 Unlike {anchorName names}`Except`, both constructors have an additional state field that includes the final state of the computation.
 
-The {anchorName names}`Monad` instance for {anchorTerm names}`EStateM ε σ` requires {anchorName names}`pure` and {anchorName names}`bind`.
-Just as with {anchorName State (module:=Examples.Monads)}`State`, the implementation of {anchorName names}`pure` for {anchorName names}`EStateM` accepts an initial state and returns it unchanged, and just as with {anchorName names}`Except`, it returns its argument in the {anchorName names (show := ok)}`EStateM.Result.ok` constructor:
+The {anchorName names}`Monad` instance for {anchorTerm names}`EST ε σ` requires {anchorName names}`pure` and {anchorName names}`bind`.
+Just as with {anchorName State (module:=Examples.Monads)}`State`, the implementation of {anchorName names}`pure` for {anchorName names}`EST` accepts an initial state and returns it unchanged, and just as with {anchorName names}`Except`, it returns its argument in the {anchorName names (show := ok)}`EST.Out.ok` constructor:
 ```anchor printEStateMpure
-#print EStateM.pure
+#print EST.pure
 ```
 ```anchorInfo printEStateMpure
-protected def EStateM.pure.{u} : {ε σ α : Type u} → α → EStateM ε σ α :=
-fun {ε σ α} a s => EStateM.Result.ok a s
+protected def EST.pure : {α ε σ : Type} → α → EST ε σ α :=
+fun {α ε σ} a s => EST.Out.ok a s
 ```
-{kw}`protected` means that the full name {anchorName printEStateMpure}`EStateM.pure` is needed even if the {anchorName names}`EStateM` namespace has been opened.
+{kw}`protected` means that the full name {anchorName printEStateMpure}`EST.pure` is needed even if the {anchorName names}`EST` namespace has been opened.
 
-Similarly, {anchorName names}`bind` for {anchorName names}`EStateM` takes an initial state as an argument.
+Similarly, {anchorName names}`bind` for {anchorName names}`EST` takes an initial state as an argument.
 It passes this initial state to its first action.
 Like {anchorName names}`bind` for {anchorName names}`Except`, it then checks whether the result is an error.
 If so, the error is returned unchanged and the second argument to {anchorName names}`bind` remains unused.
 If the result was a success, then the second argument is applied to both the returned value and to the resulting state.
 ```anchor printEStateMbind
-#print EStateM.bind
+#print EST.bind
 ```
 ```anchorInfo printEStateMbind
-protected def EStateM.bind.{u} : {ε σ α β : Type u} → EStateM ε σ α → (α → EStateM ε σ β) → EStateM ε σ β :=
+protected def EST.bind : {ε σ α β : Type} → EST ε σ α → (α → EST ε σ β) → EST ε σ β :=
 fun {ε σ α β} x f s =>
   match x s with
-  | EStateM.Result.ok a s => f a s
-  | EStateM.Result.error e s => EStateM.Result.error e s
+  | EST.Out.ok a s => f a s
+  | EST.Out.error e s => EST.Out.error e s
 ```
 
 Putting all of this together, {anchorName names}`IO` is a monad that tracks state and errors at the same time.
 The collection of available errors is that given by the datatype {anchorName printIOError}`IO.Error`, which has constructors that describe many things that can go wrong in a program.
-The state is a type that represents the real world, called {anchorTerm printRealWorld}`IO.RealWorld`.
+The state is a type that represents the real world, called {anchorTerm RealWorld}`IO.RealWorld`.
 Each basic {anchorName names}`IO` action receives this real world and returns another one, paired either with an error or a result.
 In {anchorName names}`IO`, {anchorName names}`pure` returns the world unchanged, while {anchorName names}`bind` passes the modified world from one action into the next action.
 
 Because the entire universe doesn't fit in a computer's memory, the world being passed around is just a representation.
 So long as world tokens are not re-used, the representation is safe.
-This means that world tokens do not need to contain any data at all:
-```anchor printRealWorld
-#print IO.RealWorld
-```
-```anchorInfo printRealWorld
-def IO.RealWorld : Type :=
-Unit
-```
+The type {anchorTerm RealWorld}`IO.RealWorld` is a trivial primitive type that does not need any representation at all, because it is only used inside of {anchorName VoidSigma}`Void`.
